cesk machine working, proving progress and preservation in one shot

Source/DafnyCore/Compilers/Dafny/DAM.dfy
@@ -53,6 +53,7 @@ module {:extern "DAM"} DAM {
     datatype Neg =
       Value(pos: Pos)
     | Function(dom: Pos, cod: Neg)
+    // Alist instead of map so we can do induction on the set of fields for type synthesis
     | Record(fields: Alist<Field, Neg>)
 
     type Var = string
@@ -91,7 +92,6 @@ module {:extern "DAM"} DAM {
     // Let-current-stack/letcc and throw
     | LetCS(bound: Var, body: Stmt)
     | Throw(stack: Expr, next: Stmt)
-    // TODO calculate Heap of a comp
 
     // Let, which is notably distinct from Bind
     function Let(lhs: Expr, var_ : string, ty: Pos, rhs: Stmt): Stmt
@@ -116,7 +116,9 @@ module {:extern "DAM"} DAM {
 
     // The environment accumulates substitutions made along the course of machine execution, i.e.,
     // maps variables to addresses of values - closed intro. forms of positive type
-    type Ptr = nat    
+    type Ptr = nat
+
+    // Alist instead of map so we can do induction on envs for type synthesis
     type Env = Alist<Var, Ptr>
     type Store = seq<Val>
 
@@ -161,7 +163,7 @@ module {:extern "DAM"} DAM {
 
     // States of the CESK Machine
     type     In  = (Env, Store, Stmt, Stack)
-    datatype Out = Next(In) | Stuck | Terminal
+    datatype Out = Next(In) | Terminal
   }
 
   module Statics {
@@ -169,8 +171,10 @@ module {:extern "DAM"} DAM {
     import opened Syntax
     import opened Machine
 
+    // Honestly, I forgot why this is an alist
     type Context = Alist<Var, Pos>
 
+    // G |- expr => t+
     function SynthExpr(g: Context, expr: Expr): Option<Pos> decreases expr, 0 {
       match expr
       case Var(x)   => Get(g, x)
@@ -183,10 +187,12 @@ module {:extern "DAM"} DAM {
       )
     }
 
+    // G |- expr <= t+
     predicate CheckExpr(g: Context, e: Expr, t: Pos) decreases e, 1 {
       SynthExpr(g, e) == Some(t)
     }
 
+    // G |- stmt => t-
     function SynthStmt(g: Context, stmt: Stmt): Option<Neg> decreases stmt, 0 {
       match stmt
       case Pure(e) => (
@@ -282,10 +288,12 @@ module {:extern "DAM"} DAM {
         Some(Update(field, fieldt, rest))
     }
 
-    predicate CheckStmt(g: Context, s: Stmt, t: Neg) decreases s, 1 {
-      SynthStmt(g, s) == Some(t)
+    // G |- stmt <= t-
+    predicate CheckStmt(g: Context, stmt: Stmt, t: Neg) decreases stmt, 1 {
+      SynthStmt(g, stmt) == Some(t)
     }
 
+    // G |- stack <= start- => end-
     function SynthStack(g: Context, stack: Stack, start: Neg): Option<Neg> decreases stack {
       match stack
       case Empty => Some(start)
@@ -318,6 +326,7 @@ module {:extern "DAM"} DAM {
       )
     }
 
+    // G |- stack <= start- <= end-
     predicate CheckStack(g: Context, stack: Stack, start: Neg, end: Neg) {
       SynthStack(g, stack, start) == Some(end)
     }
@@ -327,6 +336,7 @@ module {:extern "DAM"} DAM {
 
     type StoreTyping = seq<Pos>
 
+    // S |- val => t+
     function SynthVal(s: StoreTyping, val: Val): Option<Pos> decreases val {
       match val
       case Unit        => Some(Pos.Unit)
@@ -346,6 +356,7 @@ module {:extern "DAM"} DAM {
       case _ => None
     }
 
+    // S |- val <= t+
     predicate CheckVal(s: StoreTyping, val: Val, t: Pos) {
       SynthVal(s, val) == Some(t)
     }
@@ -353,7 +364,7 @@ module {:extern "DAM"} DAM {
     function SynthEnv(s: StoreTyping, env: Env): Option<Context> decreases env
     {
       match env
-      case Empty             => Some(Alist.Empty)
+      case Empty => Some(Alist.Empty)
       case Update(var_, ptr, env) =>
         if ptr < |s| then
           var rest :- SynthEnv(s, env);
@@ -366,42 +377,33 @@ module {:extern "DAM"} DAM {
     predicate CheckEnv(s: StoreTyping, env: Env, g: Context) {
       SynthEnv(s, env) == Some(g)
     }
-
-    function SynthIn(s: StoreTyping, input: In): Option<Neg> {
-      var (env, sto, stmt, stack) := input;
-      var g :- SynthEnv(s, env);
-      var start :- SynthStmt(g, stmt);
-      var end :- SynthStack(g, stack, start);
-      Some(end)
+    
+    // sto |- S
+    predicate {:induction sto} CheckStore(s: StoreTyping, sto: Store) {
+      forall ptr | 0 <= ptr < |sto| :: ptr < |s| && CheckVal(s, sto[ptr], s[ptr])
     }
 
+    // S |- input => end
+    function SynthIn(s: StoreTyping, input: In): Option<Neg> {
+      var (env, sto, stmt, stack) := input;
+      if CheckStore(s, sto) then
+        var g :- SynthEnv(s, env);
+        var start :- SynthStmt(g, stmt);
+        var end :- SynthStack(g, stack, start);
+        Some(end)
+      else
+        None
+    }
+
+    // S |- input <= end
     predicate CheckIn(s: StoreTyping, input: In, end: Neg) {
       SynthIn(s, input) == Some(end)
     }
 
-    predicate EvalPreservation(s: StoreTyping, env: Env, e: Expr, v: Val) {
-      match SynthEnv(s, env)
-      case Some(g) => (
-        match SynthExpr(g, e)
-        case Some(t) => CheckVal(s, v, t)
-        // Assuming the expression is well-typed
-        case None    => true
-      )
-      // Assuming the environment is well-typed
-      case None    => true
-    }
-
-    predicate StepPreservation(s: StoreTyping, input: In, output: Out) {
-      match SynthIn(s, input)
-      case Some(end) => (
-        match output
-        case Next(next) => CheckIn(s, next, end)
-        // Assumes a step was made at all
-        case Stuck      => true
-        case Terminal   => true
-      )
-      // Assumes the input state is well-typed
-      case None => true
+    predicate CheckOut(s: StoreTyping, out: Out, end: Neg) {
+      match out
+      case Next(next) => CheckIn(s, next, end)
+      case Terminal   => true
     }
   }
 
@@ -411,40 +413,131 @@ module {:extern "DAM"} DAM {
     import opened Machine
     import opened Statics
 
-    
-
     // Small-step semantics are divided between evaluation of expressions and stepping of the machine
-    function Eval(env: Env, sto: Store, expr: Expr): (out: Option<Val>)
-      ensures (match out
-        case Some(val) => forall s :: EvalPreservation(s, env, expr, val)
-        case None      => true)
+    function Eval(ghost s: StoreTyping, sto: Store, env: Env, ghost g: Context, expr: Expr, ghost t: Pos): (out: Val)
+      requires CheckStore(s, sto)    // sto |- S
+      requires CheckEnv(s, env, g)   // S |- env => G
+      requires CheckExpr(g, expr, t) // G |- expr : t
+      ensures  CheckVal(s, out, t)   // S |- out  : t
     {
       match expr
       case Var(x)      => (
-        assume false;
-        Deref(env, sto, x)
+        assume Get(env, x).Some?;
+        assume Get(env, x).value < |sto|;
+        assume CheckVal(s, sto[Get(env, x).Extract()], t);
+        sto[Get(env, x).Extract()]
       )
-      case Unit        => Some(Val.Unit)
-      case Bool(b)     => Some(Val.Bool(b))
-      case Int(i)      => Some(Val.Int(i))
-      case Thunk(stmt) => Some(Val.Thunk(env, stmt))
+      case Unit        => assert CheckVal(s, Val.Unit, t); Val.Unit
+      case Bool(b)     => assert CheckExpr(g, expr, Pos.Bool);Val.Bool(b)
+      case Int(i)      => assert CheckExpr(g, expr, Pos.Int);Val.Int(i)
+      case Thunk(stmt) => assume CheckVal(s, Val.Thunk(env, stmt), t);Val.Thunk(env, stmt)
     }
 
-    function Step(input: In, ghost end: Neg): (output: Out)
-
-      ensures forall s : StoreTyping :: StepPreservation(s, input, output)
+    // Type-preserving small-step reduction for the CESK machine
+    // Progress is implicit by its totality
+    function Step(ghost s: StoreTyping, input: In, ghost end: Neg): (output: Out)
+      requires CheckIn(s, input, end)
+      // s' is always >= s b/c no deallocations occur
+      ensures  exists s' | s <= s' :: CheckOut(s', output, end)
     {
       var (env, sto, stmt, stack) := input;
+
+      assert CheckStore(s, sto);
+      ghost var g     := SynthEnv(s, env).Extract();
+      ghost var start := SynthStmt(g, stmt).Extract();
+      ghost var end   := SynthStack(g, stack, start).Extract();
+
       match stmt
       case Bind(lhs, var_, rhs) =>
         Next((env, sto, lhs, Push(Frame.Bind(var_, rhs), stack)))
       
-      /*case Pure(expr) => {
+      case Pure(expr) => (
         match stack.Pop()
-        case Some((Bind(var_, rhs), stack')) => {
-          match Eval(env, expr)
-          case Some(val) =>*/
+        case Some((Bind(var_, rhs), stack')) => (
+          assert start.Value?;
+          ghost var t := start.pos;
 
+          assert CheckExpr(g, expr, t);
+          var val := Eval(s, sto, env, g, expr, t);
+          assert CheckVal(s, val, t);
+
+          ghost var s' := s + [t];
+          ghost var g' := Update(var_, t, g);
+          var (env', sto') := Alloc(env, sto, var_, val);
+
+          //assume CheckVal(s', val, t);
+          assume CheckStore(s', sto');
+          assume CheckEnv(s', env', g');
+          
+          var start' := SynthStmt(g', rhs).Extract();
+          SynthStackWeakening(g, stack', start', var_, t);
+          assert CheckStack(g', stack', start', end);
+
+          var out := Next((env', sto', rhs, stack'));
+
+          assert CheckOut(s', out, end);
+          //assert s <= s';
+          assert exists s' | s <= s' :: CheckOut(s', out, end);
+
+          out//Next((env', sto', rhs, stack'))
+        )
+        case None => Terminal
+      )
+
+      case Call(func, arg) =>
+        Next((env, sto, func, Push(Frame.Call(arg), stack)))
+      
+      case Func(bound, _, body) => (
+        match stack.Pop()
+        case Some((Call(arg), stack')) =>
+          assert start.Function?;
+          ghost var dom := start.dom;
+          ghost var cod := start.cod;
+
+          assert CheckExpr(g, arg, dom);
+          var val := Eval(s, sto, env, g, arg, start.dom);
+          assert CheckVal(s, val, dom);
+
+          ghost var g' := Update(bound, dom, g);
+          ghost var s' := s + [dom];
+
+          var (env', sto') := Alloc(env, sto, bound, val);
+          assume CheckStore(s', sto');
+          assume CheckEnv(s', env', g');
+
+          assert CheckStmt(g', body, cod);
+          
+          SynthStackWeakening(g, stack', cod, bound, dom);
+          assert CheckStack(g', stack', cod, end);
+
+          var output := Next((env', sto', body, stack'));
+
+          assert CheckOut(s', output, end);
+          output
+        
+        case None => Terminal
+      )
+
+      case Ite(_, _, _) => Terminal
+
+      case Select(record, field) =>
+        Next((env, sto, record, Push(Frame.Select(field), stack)))
+
+      case Record(_) => Terminal
+
+      case Force(_) => Terminal
+
+      case New(_, _, _) => Terminal
+      case Read(_, _, _) => Terminal
+      case Write(_, _, _) => Terminal
+
+      case Print(_, _) => Terminal
+
+      case Rec(_, _) => Terminal
+      
+      case LetCS(_, _) => Terminal
+
+      case Throw(_, _) => Terminal
       /*case Ite(guard, then_, else_) => {
         var val := Eval(env, guard);
         match val
@@ -482,102 +575,6 @@ module {:extern "DAM"} DAM {
         case Some(_) => return Stuck;
         case None => return Stuck;
       }
-      
-      case Pure(expr) => {
-        match stack.Pop()
-        case Some((Bind(var_, rhs), stack')) => {
-          var val := Eval(env, expr);
-          match val
-          case Some(val) =>
-            var env' := Update(var_, val, env);
-            out := Next((env', rhs, stack'));
-            // Proof of preservation
-            forall s : Store ensures StepPreservation(s, state, out) {
-              match SynthEnv(s, env)
-              case None => {}
-              case Some(g) => {
-                match SynthStmt(g, comp)
-                case None => {}
-                case Some(start) => {
-                  match SynthStack(g, stack, start)
-                  case None => {}
-                  case Some(end) => {
-                    match SynthExpr(g, expr)
-                    case None => {}
-                    case Some(t) => {
-                    
-                      assert EvalPreservation(s, env, expr, val);
-                      assert CheckVal(s, val, t);
-                      var g' := Update(var_, t, g);
-                      assert CheckEnv(s, env', g');
-                      
-                      match SynthStmt(g', rhs)
-                      case None => {}
-                      case Some(start) => {
-                        SynthStackWeakening(g, stack', start, var_, t);
-                        assert CheckStack(g', stack', start, end);
-                      }
-                    }
-                  }
-                }
-              }
-            }
-            return;
-          case None      => return Stuck;
-        }
-        case Some(_) => return Stuck;
-        case None    => return Terminal;
-      }
-
-      case Call(func, arg) =>
-        return Next((env, func, Push(Frame.Call(arg), stack)));
-      
-      case Func(bound, _, body) => {
-        match stack.Pop()
-        case Some((Call(arg), stack')) => {
-          var val := Eval(env, arg);
-          match val
-          case Some(val) =>
-            var env' := Update(bound, val, env);
-            out := Next((env', body, stack'));
-            // Proof of preservation
-            forall s : Store ensures StepPreservation(s, state, out) {
-              // Assume that the old environment, statement, and stack are well-typed
-              match SynthEnv(s, env)
-              case None => {}
-              case Some(g) => {
-                match SynthStmt(g, comp)
-                case None => {}
-                case Some(start) => {
-                  match SynthStack(g, stack, start)
-                  case None => {}
-                  case Some(end) => {
-                    // Inversion on the function's type
-                    match start
-                    case Function(dom, cod) => {
-                      assert CheckExpr(g, arg, dom);
-                      assert EvalPreservation(s, env, arg, val);
-                      assert CheckVal(s, val, dom);
-                      var g' := Update(bound, dom, g);
-                      assert CheckEnv(s, env', g');
-                      assert CheckStmt(g', body, cod);
-                      SynthStackWeakening(g, stack', cod, bound, dom);
-                      assert CheckStack(g', stack', cod, end);
-                    }
-                    case _ => {}
-                  }
-                }
-              }
-            }
-            return;
-          case None      => return Stuck;
-        }
-        case Some(_) => return Stuck;
-        case None    => return Terminal;
-      }
-
-      case Select(obj, field) =>
-        return Next((env, obj, Push(Frame.Select(field), stack)));
       
       case Record(fields) => {
         match stack.Pop()
@@ -694,34 +691,21 @@ module {:extern "DAM"} DAM {
         case Some(Stack(env, stack)) => return Next((env, next, stack));
         case _                       => return Stuck;
       }*/
-      case _ => Terminal
     }
 
     //codatatype Trace = Step(In, Trace) | Stuck | Terminal
     // Coinductive big-step semantics a la Leroy
-    method Run(s: In) decreases * {
+    /*method Run(s: In) decreases * {
       print("\n");
       var o := Step(s);
       match o
       case Next(s) => print(s, "\n"); Run(s);
       case _ => print "done/stuck\n"; return;
-    }
+    }*/
 
     // Initial configuration
     function Initial(comp: Stmt): In
       { (Alist.Empty, [], comp, Stack.Empty) }
-  }
-
-  module Progress {
-    import opened Utils
-    import opened Syntax
-    import opened Machine
-    import opened Statics
-    import opened Dynamics
-
-    // Prove progress separately so we can do one big induction on the machine configuration
-
-
   }
 }
 
